Challenge/Ripemd160/Submission/Proofs/Bytecode/GuardInstructionWindow.lean
@@ -66,7 +66,7 @@ def tail : List Instr :=
   op 0x36,
   op 0x8c,
   op 0x14,
-  .push 2 4712,
+  .push 2 4710,
   op 0x57,
   op 0x50,
   op 0x50,
@@ -135,7 +135,7 @@ def tail : List Instr :=
   op 0x1c,
   op 0x90,
   op 0x81,
-  .push 2 4689,
+  .push 2 4687,
   op 0x57,
   op 0x50,
   op 0x50,
@@ -146,12 +146,9 @@ def tail : List Instr :=
   op 0x36,
   .push 0 0,
   op 0x37,
-  .push 1 128,
   op 0x36,
   .push 1 3,
   op 0x1b,
-  op 0x5b,
-  op 0x5b,
   op 0x80,
   .push 1 162,
   op 0x52,
@@ -160,19 +157,17 @@ def tail : List Instr :=
   op 0x52,
   .push 1 144,
   op 0x52,
-  op 0x80,
+  .push 1 128,
   .push 2 522,
   op 0x52,
-  op 0x80,
+  .push 19 2854495385411919762116571938898990272765493376,
   .push 1 54,
-  op 0x52,
-  .push 1 36,
   op 0x52,
   op 0x36,
   .push 1 29,
   op 0x1c,
   op 0x15,
-  .push 2 908,
+  .push 2 906,
   op 0x57,
   op 0x36,
   .push 1 29,
@@ -191,7 +186,7 @@ def tail : List Instr :=
   op 0x52,
   .push 2 270,
   op 0x52,
-  .push 2 908,
+  .push 2 906,
   op 0x56,
   op 0x5b,
   .push 17 342276208914615837337402008677671501826,
@@ -233,21 +228,21 @@ def tail : List Instr :=
   op 0x52,
   op 0x59,
   .push 0 0,
-  op 0xf3,
+  op 0xf3
 ]
-theorem tail_eq : Artifact.submissionArtifact.instructions.drop 3596 = tail := by rfl
+theorem tail_eq : Artifact.submissionArtifact.instructions.drop 3594 = tail := by rfl
 
-theorem pc_base : Artifact.submissionArtifact.instructionPC 3596 = 4508 := by
+theorem pc_base : Artifact.submissionArtifact.instructionPC 3594 = 4506 := by
   rw [instructionPC_eq_byteLength]
   rfl
 
 theorem get (index : Nat) :
-    Artifact.submissionArtifact.instructions[3596 + index]? = tail[index]? := by
+    Artifact.submissionArtifact.instructions[3594 + index]? = tail[index]? := by
   rw [← InstructionWindow.get_drop, tail_eq]
 
 theorem pc (index : Nat) :
-    Artifact.submissionArtifact.instructionPC (3596 + index) =
-      4508 + byteLength (tail.take index) := by
+    Artifact.submissionArtifact.instructionPC (3594 + index) =
+      4506 + byteLength (tail.take index) := by
   rw [InstructionWindow.pc_drop, pc_base, tail_eq]
 
 #print axioms get
